Starting to incorporate the host correctness.

theories/host.v
@@ -3,7 +3,7 @@
 
 From mathcomp Require Import ssreflect ssrfun ssrnat ssrbool eqtype seq.
 Require Import common datatypes.
-From ExtLib Require Import Monad.
+From Prelude Require Import Classes.
 
 Set Implicit Arguments.
 
@@ -28,53 +28,67 @@ Record host := {
     host_state : eqType ;
     host_application : host_state -> store_record -> host_function -> seq value ->
                        host_state -> option (store_record * result) -> Prop
-    (* FIXME: Should the resulting [host_state] be part of the [option]? *)
+    (* FIXME: Should the resulting [host_state] be part of the [option]?
+      (See https://github.com/rems-project/wasm_coq/issues/16#issuecomment-616402508
+       for a discussion about this.) *)
   }.
 
 Record monadic_host := {
     host_monad : Type -> Type ;
-    host_Monad : Monad host_monad ;
+    host_Monad :> Monad host_monad ;
     host_apply : store_record -> host_function -> seq value ->
                  host_monad (option (store_record * result))
   }.
+
+Global Instance monadic_host_Monad : forall mh, Monad (host_monad mh).
+Proof. move=> mh. exact mh. Defined.
 
 (** We introduce this structure to be able to reason about monads,
   and in particular to be able to relate a monadic interpreter with
   a usual small-step semantics.
   It is based on a special high-order predicate that transpose a
   predicate about inside the monad. **)
-Record ReasonMonad m (M : Monad m) := {
+Class ReasonMonad m (M : Monad m) := {
     reason_predicate : forall A : Type, (A -> Prop) -> m A -> Prop ;
-    reason_predicate_ret : forall A (p : A -> Prop) (a : A), p a -> reason_predicate p (ret a) ;
+    reason_predicate_pure : forall A (p : A -> Prop) (a : A), p a -> reason_predicate p (pure a) ;
     reason_predicate_bind : forall A B (p : A -> Prop) (q : B -> Prop) (f : A -> m B) (m : m A),
       (forall a : A, p a -> reason_predicate q (f a)) ->
       reason_predicate p m ->
-      reason_predicate q (bind m f)
+      reason_predicate q (m >>= f)%monad
   }.
 Arguments ReasonMonad m {M}.
 
-(** In particular, any injective monad can be reasonned as-is. **)
-Program Definition injective_ReasonMonad : forall m (M : Monad m),
-  (forall A, injective (ret : A -> m A)) ->
-  ReasonMonad m :=
-  fun m M I => {|
-      reason_predicate := fun A p m => forall r, m = ret r -> p r
+(** In particular, some monads can be reversed. **)
+Class ReversibleMonad m (M : Monad m) := {
+    reversible_pure : forall A, injective (pure (a := _) : A -> m A) ;
+    reversible_bind : forall A B (f : A -> m B) (m : m A) (b : B),
+      (m >>= f)%monad = pure b ->
+      exists a, m = pure a /\ f a = pure b
+  }.
+Arguments ReversibleMonad m {M}.
+
+(** Any reversible monad comes with a natural way to reason on it. **)
+Instance ReversibleMonad_ReasonMonad : forall m (M : Monad m),
+  ReversibleMonad m ->
+  ReasonMonad m.
+Proof.
+  move=> m M RM.
+  refine {|
+      reason_predicate := fun A p m => forall r, m = pure r -> p r
     |}.
-Next Obligation.
-  apply I in H0. by subst.
-Qed.
-Next Obligation.
-  admit (* FIXME: Where are the axioms on [bind]? *)
-Qed.
+  - move=> > ? > H. apply reversible_pure in H => //. by subst.
+  - move=> > Rf Rp > E. apply reversible_bind in E => //. move: E => [a [E1 E2]].
+    apply: Rf E2. by apply: Rp E1.
+Defined.
 
 (** Relation between [monadic_host] and [host]. **)
-
-(* TODO *)
+Record monad_host_match (h : host) (mh : monadic_host) := {
+    host_reason : ReasonMonad (host_monad mh)
+    (* TODO: Can we make it a reader monad just there? *)
+  }.
 
 End Parameterised.
 
 Arguments host_application [_ _].
-
-Arguments host_return [_ _ _].
-Arguments host_bind [_ _ _ _].
 Arguments host_apply [_ _].
+
