theories/interpreter.v
@@ -5,6 +5,7 @@ Require Import common.
 From Coq Require Import ZArith.BinInt.
 From mathcomp Require Import ssreflect ssrfun ssrnat ssrbool eqtype seq.
 Require Export operations host type_checker.
+From Prelude Require Import Control.
 
 Set Implicit Arguments.
 Unset Strict Implicit.
@@ -151,27 +152,29 @@ Proof.
   - move=> >. by apply: ReflectF.
 Qed.
 
+Open Scope monad.
+
 Fixpoint run_step_with_fuel (fuel : fuel) (d : depth) (i : instance) (tt : config_tuple)
     : host_monad res_tuple :=
   let: (s, vs, es) := tt in
   match fuel with
-  | 0 => host_return (s, vs, RS_crash C_exhaustion)
+  | 0 => pure (s, vs, RS_crash C_exhaustion)
   | fuel.+1 =>
     let: (ves, es') := split_vals_e es in (** Framing out constants. **)
     match es' with
-    | [::] => host_return (s, vs, crash_error)
+    | [::] => pure (s, vs, crash_error)
     | e :: es'' =>
       if e_is_trap e
       then
         if (es'' != [::]) || (ves != [::])
-        then host_return (s, vs, RS_normal [::Trap])
-        else host_return (s, vs, crash_error)
+        then pure (s, vs, RS_normal [::Trap])
+        else pure (s, vs, crash_error)
       else
-        host_bind (run_one_step fuel d i (s, vs, (rev ves)) e) (fun rosf =>
+        bind (run_one_step fuel d i (s, vs, (rev ves)) e) (fun rosf =>
           let: (s', vs', r) := rosf in
           if r is RS_normal res
-          then host_return (s', vs', RS_normal (res ++ es''))
-          else host_return (s', vs', r))
+          then pure (s', vs', RS_normal (res ++ es''))
+          else pure (s', vs', r))
     end
   end
 
@@ -179,88 +182,88 @@ with run_one_step (fuel : fuel) (d : depth) (i : instance) (tt : config_one_tupl
     : host_monad res_tuple :=
   let: (s, vs, ves) := tt in
   match fuel with
-  | 0 => host_return (s, vs, RS_crash C_exhaustion)
+  | 0 => pure (s, vs, RS_crash C_exhaustion)
   | fuel.+1 =>
     match e with
 
     (** unop **)
     | Basic (Unop_i T_i32 iop) =>
       if ves is ConstInt32 c :: ves' then
-        host_return (s, vs, RS_normal (vs_to_es ((ConstInt32 (@app_unop_i i32t iop c)) :: ves')))
-      else host_return (s, vs, crash_error)
+        pure (s, vs, RS_normal (vs_to_es ((ConstInt32 (@app_unop_i i32t iop c)) :: ves')))
+      else pure (s, vs, crash_error)
     | Basic (Unop_i T_i64 iop) =>
       if ves is (ConstInt64 c) :: ves' then
-        host_return (s, vs, RS_normal (vs_to_es ((ConstInt64 (@app_unop_i i64t iop c)) :: ves')))
-      else host_return (s, vs, crash_error)
-    | Basic (Unop_i _ _) => host_return (s, vs, crash_error)
+        pure (s, vs, RS_normal (vs_to_es ((ConstInt64 (@app_unop_i i64t iop c)) :: ves')))
+      else pure (s, vs, crash_error)
+    | Basic (Unop_i _ _) => pure (s, vs, crash_error)
     | Basic (Unop_f T_f32 iop) =>
       if ves is (ConstFloat32 c) :: ves' then
-        host_return (s, vs, RS_normal (vs_to_es ((ConstFloat32 (@app_unop_f f32t iop c)) :: ves')))
-      else host_return (s, vs, crash_error)
+        pure (s, vs, RS_normal (vs_to_es ((ConstFloat32 (@app_unop_f f32t iop c)) :: ves')))
+      else pure (s, vs, crash_error)
     | Basic (Unop_f T_f64 iop) =>
       if ves is (ConstFloat64 c) :: ves' then
-        host_return (s, vs, RS_normal (vs_to_es ((ConstFloat64 (@app_unop_f f64t iop c)) :: ves')))
-      else host_return (s, vs, crash_error)
-    | Basic (Unop_f _ _) => host_return (s, vs, crash_error)
+        pure (s, vs, RS_normal (vs_to_es ((ConstFloat64 (@app_unop_f f64t iop c)) :: ves')))
+      else pure (s, vs, crash_error)
+    | Basic (Unop_f _ _) => pure (s, vs, crash_error)
 
     (** binop **)
     | Basic (Binop_i T_i32 iop) =>
       if ves is (ConstInt32 c2) :: (ConstInt32 c1) :: ves' then
         expect (@app_binop_i i32t iop c1 c2) (fun c =>
-            host_return (s, vs, RS_normal (vs_to_es ((ConstInt32 c) :: ves'))))
-          (host_return (s, vs, RS_normal ((vs_to_es ves') ++ [::Trap])))
-      else host_return (s, vs, crash_error)
+            pure (s, vs, RS_normal (vs_to_es ((ConstInt32 c) :: ves'))))
+          (pure (s, vs, RS_normal ((vs_to_es ves') ++ [::Trap])))
+      else pure (s, vs, crash_error)
     | Basic (Binop_i T_i64 iop) =>
       if ves is (ConstInt64 c2) :: (ConstInt64 c1) :: ves' then
         expect (@app_binop_i i64t iop c1 c2) (fun c =>
-            host_return (s, vs, RS_normal (vs_to_es ((ConstInt64 c) :: ves'))))
-          (host_return (s, vs, RS_normal ((vs_to_es ves') ++ [::Trap])))
-      else host_return (s, vs, crash_error)
-    | Basic (Binop_i _ _) => host_return (s, vs, crash_error)
+            pure (s, vs, RS_normal (vs_to_es ((ConstInt64 c) :: ves'))))
+          (pure (s, vs, RS_normal ((vs_to_es ves') ++ [::Trap])))
+      else pure (s, vs, crash_error)
+    | Basic (Binop_i _ _) => pure (s, vs, crash_error)
     | Basic (Binop_f T_f32 fop) =>
       if ves is (ConstFloat32 c2) :: (ConstFloat32 c1) :: ves' then
         expect (@app_binop_f f32t fop c1 c2) (fun c =>
-            host_return (s, vs, RS_normal (vs_to_es ((ConstFloat32 c) :: ves'))))
-          (host_return (s, vs, RS_normal ((vs_to_es ves') ++ [::Trap])))
-      else host_return (s, vs, crash_error)
+            pure (s, vs, RS_normal (vs_to_es ((ConstFloat32 c) :: ves'))))
+          (pure (s, vs, RS_normal ((vs_to_es ves') ++ [::Trap])))
+      else pure (s, vs, crash_error)
     | Basic (Binop_f T_f64 fop) =>
       if ves is (ConstFloat64 c2) :: (ConstFloat64 c1) :: ves' then
         expect (@app_binop_f f64t fop c1 c2) (fun c =>
-             host_return (s, vs, RS_normal (vs_to_es ((ConstFloat64 c) :: ves'))))
-          (host_return (s, vs, RS_normal ((vs_to_es ves') ++ [::Trap])))
-      else host_return (s, vs, crash_error)
-    | Basic (Binop_f _ _) => host_return (s, vs, crash_error)
+             pure (s, vs, RS_normal (vs_to_es ((ConstFloat64 c) :: ves'))))
+          (pure (s, vs, RS_normal ((vs_to_es ves') ++ [::Trap])))
+      else pure (s, vs, crash_error)
+    | Basic (Binop_f _ _) => pure (s, vs, crash_error)
 
     (** testops **)
     | Basic (Testop T_i32 testop) =>
       if ves is (ConstInt32 c) :: ves' then
-        host_return (s, vs, RS_normal (vs_to_es ((ConstInt32 (wasm_bool (@app_testop_i i32t testop c))) :: ves')))
-      else host_return (s, vs, crash_error)
+        pure (s, vs, RS_normal (vs_to_es ((ConstInt32 (wasm_bool (@app_testop_i i32t testop c))) :: ves')))
+      else pure (s, vs, crash_error)
     | Basic (Testop T_i64 testop) =>
       if ves is (ConstInt64 c) :: ves' then
-        host_return (s, vs, RS_normal (vs_to_es ((ConstInt32 (wasm_bool (@app_testop_i i64t testop c))) :: ves')))
-      else host_return (s, vs, crash_error)
-    | Basic (Testop _ _) => host_return (s, vs, crash_error)
+        pure (s, vs, RS_normal (vs_to_es ((ConstInt32 (wasm_bool (@app_testop_i i64t testop c))) :: ves')))
+      else pure (s, vs, crash_error)
+    | Basic (Testop _ _) => pure (s, vs, crash_error)
 
     (** relops **)
     | Basic (Relop_i T_i32 iop) =>
       if ves is (ConstInt32 c2) :: (ConstInt32 c1) :: ves' then
-        host_return (s, vs, RS_normal (vs_to_es (ConstInt32 (wasm_bool (@app_relop_i i32t iop c1 c2)) :: ves')))
-      else host_return (s, vs, crash_error)
+        pure (s, vs, RS_normal (vs_to_es (ConstInt32 (wasm_bool (@app_relop_i i32t iop c1 c2)) :: ves')))
+      else pure (s, vs, crash_error)
     | Basic (Relop_i T_i64 iop) =>
       if ves is (ConstInt64 c2) :: (ConstInt64 c1) :: ves' then
-        host_return (s, vs, RS_normal (vs_to_es (ConstInt32 (wasm_bool (@app_relop_i i64t iop c1 c2)) :: ves')))
-      else host_return (s, vs, crash_error)
-    | Basic (Relop_i _ _) => host_return (s, vs, crash_error)
+        pure (s, vs, RS_normal (vs_to_es (ConstInt32 (wasm_bool (@app_relop_i i64t iop c1 c2)) :: ves')))
+      else pure (s, vs, crash_error)
+    | Basic (Relop_i _ _) => pure (s, vs, crash_error)
     | Basic (Relop_f T_f32 iop) =>
       if ves is (ConstFloat32 c2) :: (ConstFloat32 c1) :: ves' then
-        host_return (s, vs, RS_normal (vs_to_es (ConstInt32 (wasm_bool (@app_relop_f f32t iop c1 c2)) :: ves')))
-      else host_return (s, vs, crash_error)
+        pure (s, vs, RS_normal (vs_to_es (ConstInt32 (wasm_bool (@app_relop_f f32t iop c1 c2)) :: ves')))
+      else pure (s, vs, crash_error)
     | Basic (Relop_f T_f64 iop) =>
       if ves is (ConstFloat64 c2) :: (ConstFloat64 c1) :: ves' then
-        host_return (s, vs, RS_normal (vs_to_es (ConstInt32 (wasm_bool (@app_relop_f f64t iop c1 c2)) :: ves')))
-      else host_return (s, vs, crash_error)
-    | Basic (Relop_f _ _) => host_return (s, vs, crash_error)
+        pure (s, vs, RS_normal (vs_to_es (ConstInt32 (wasm_bool (@app_relop_f f64t iop c1 c2)) :: ves')))
+      else pure (s, vs, crash_error)
+    | Basic (Relop_f _ _) => pure (s, vs, crash_error)
 
     (** convert and reinterpret **)
     | Basic (Cvtop t2 Convert t1 sx) =>
@@ -268,110 +271,110 @@ with run_one_step (fuel : fuel) (d : depth) (i : instance) (tt : config_one_tupl
         if types_agree t1 v
         then
           expect (cvt t2 sx v) (fun v' =>
-               host_return (s, vs, RS_normal (vs_to_es (v' :: ves'))))
-            (host_return (s, vs, RS_normal ((vs_to_es ves') ++ [::Trap])))
-        else host_return (s, vs, crash_error)
-      else host_return (s, vs, crash_error)
+               pure (s, vs, RS_normal (vs_to_es (v' :: ves'))))
+            (pure (s, vs, RS_normal ((vs_to_es ves') ++ [::Trap])))
+        else pure (s, vs, crash_error)
+      else pure (s, vs, crash_error)
     | Basic (Cvtop t2 Reinterpret t1 sx) =>
       if ves is v :: ves' then
         if types_agree t1 v && (sx == None)
-        then host_return (s, vs, RS_normal (vs_to_es (wasm_deserialise (bits v) t2 :: ves')))
-        else host_return (s, vs, crash_error)
-      else host_return (s, vs, crash_error)
+        then pure (s, vs, RS_normal (vs_to_es (wasm_deserialise (bits v) t2 :: ves')))
+        else pure (s, vs, crash_error)
+      else pure (s, vs, crash_error)
 
     (** control-flow instructions **)
-    | Basic Unreachable => host_return (s, vs, RS_normal ((vs_to_es ves) ++ [::Trap]))
-    | Basic Nop => host_return (s, vs, RS_normal (vs_to_es ves))
+    | Basic Unreachable => pure (s, vs, RS_normal ((vs_to_es ves) ++ [::Trap]))
+    | Basic Nop => pure (s, vs, RS_normal (vs_to_es ves))
     | Basic Drop =>
       if ves is v :: ves' then
-        host_return (s, vs, RS_normal (vs_to_es ves'))
-      else host_return (s, vs, crash_error)
+        pure (s, vs, RS_normal (vs_to_es ves'))
+      else pure (s, vs, crash_error)
     | Basic Select =>
       if ves is (ConstInt32 c) :: v2 :: v1 :: ves' then
         if c == Wasm_int.int_zero i32m
-        then host_return (s, vs, RS_normal (vs_to_es (v2 :: ves')))
-        else host_return (s, vs, RS_normal (vs_to_es (v1 :: ves')))
-      else host_return (s, vs, crash_error)
+        then pure (s, vs, RS_normal (vs_to_es (v2 :: ves')))
+        else pure (s, vs, RS_normal (vs_to_es (v1 :: ves')))
+      else pure (s, vs, crash_error)
     | Basic (Block (Tf t1s t2s) es) =>
       if length ves >= length t1s
       then
         let: (ves', ves'')  := split_n ves (length t1s) in
-        host_return (s, vs, RS_normal (vs_to_es ves''
+        pure (s, vs, RS_normal (vs_to_es ves''
                               ++ [::Label (length t2s) [::] (vs_to_es ves' ++ to_e_list es)]))
-      else host_return (s, vs, crash_error)
+      else pure (s, vs, crash_error)
     | Basic (Loop (Tf t1s t2s) es) =>
       if length ves >= length t1s
       then
         let: (ves', ves'') := split_n ves (length t1s) in
-        host_return (s, vs, RS_normal (vs_to_es ves''
+        pure (s, vs, RS_normal (vs_to_es ves''
                               ++ [::Label (length t1s) [::Basic (Loop (Tf t1s t2s) es)]
                                       (vs_to_es ves' ++ to_e_list es)]))
-      else host_return (s, vs, crash_error)
+      else pure (s, vs, crash_error)
     | Basic (If tf es1 es2) =>
       if ves is ConstInt32 c :: ves' then
         if c == Wasm_int.int_zero i32m
-        then host_return (s, vs, RS_normal (vs_to_es ves' ++ [::Basic (Block tf es2)]))
-        else host_return (s, vs, RS_normal (vs_to_es ves' ++ [::Basic (Block tf es1)]))
-      else host_return (s, vs, crash_error)
-    | Basic (Br j) => host_return (s, vs, RS_break j ves)
+        then pure (s, vs, RS_normal (vs_to_es ves' ++ [::Basic (Block tf es2)]))
+        else pure (s, vs, RS_normal (vs_to_es ves' ++ [::Basic (Block tf es1)]))
+      else pure (s, vs, crash_error)
+    | Basic (Br j) => pure (s, vs, RS_break j ves)
     | Basic (Br_if j) =>
       if ves is ConstInt32 c :: ves' then
         if c == Wasm_int.int_zero i32m
-        then host_return (s, vs, RS_normal (vs_to_es ves'))
-        else host_return (s, vs, RS_normal (vs_to_es ves' ++ [::Basic (Br j)]))
-      else host_return (s, vs, crash_error)
+        then pure (s, vs, RS_normal (vs_to_es ves'))
+        else pure (s, vs, RS_normal (vs_to_es ves' ++ [::Basic (Br j)]))
+      else pure (s, vs, crash_error)
     | Basic (Br_table js j) =>
       if ves is ConstInt32 c :: ves' then
         let: k := Wasm_int.nat_of_uint i32m c in
         if k < length js
         then
-          host_return (expect (List.nth_error js k) (fun js_at_k =>
+          pure (expect (List.nth_error js k) (fun js_at_k =>
               (s, vs, RS_normal (vs_to_es ves' ++ [::Basic (Br js_at_k)])))
             (s, vs, crash_error))
-        else host_return (s, vs, RS_normal (vs_to_es ves' ++ [::Basic (Br j)]))
-      else host_return (s, vs, crash_error)
+        else pure (s, vs, RS_normal (vs_to_es ves' ++ [::Basic (Br j)]))
+      else pure (s, vs, crash_error)
     | Basic (Call j) =>
       if sfunc s i j is Some sfunc_i_j then
-        host_return (s, vs, RS_normal (vs_to_es ves ++ [::Callcl sfunc_i_j]))
-      else host_return (s, vs, crash_error)
+        pure (s, vs, RS_normal (vs_to_es ves ++ [::Callcl sfunc_i_j]))
+      else pure (s, vs, crash_error)
     | Basic (Call_indirect j) =>
       if ves is ConstInt32 c :: ves' then
         match stab s i (Wasm_int.nat_of_uint i32m c) with
         | Some cl =>
           if stypes s i j == Some (cl_type cl)
-          then host_return (s, vs, RS_normal (vs_to_es ves' ++ [::Callcl cl]))
-          else host_return (s, vs, RS_normal (vs_to_es ves' ++ [::Trap]))
-        | None => host_return (s, vs, RS_normal (vs_to_es ves' ++ [::Trap]))
+          then pure (s, vs, RS_normal (vs_to_es ves' ++ [::Callcl cl]))
+          else pure (s, vs, RS_normal (vs_to_es ves' ++ [::Trap]))
+        | None => pure (s, vs, RS_normal (vs_to_es ves' ++ [::Trap]))
         end
-      else host_return (s, vs, crash_error)
-    | Basic Return => host_return (s, vs, RS_return ves)
+      else pure (s, vs, crash_error)
+    | Basic Return => pure (s, vs, RS_return ves)
     | Basic (Get_local j) =>
       if j < length vs
       then
-        host_return (expect (List.nth_error vs j) (fun vs_at_j =>
+        pure (expect (List.nth_error vs j) (fun vs_at_j =>
             (s, vs, RS_normal (vs_to_es (vs_at_j :: ves))))
           (s, vs, crash_error))
-      else host_return (s, vs, crash_error)
+      else pure (s, vs, crash_error)
     | Basic (Set_local j) =>
       if ves is v :: ves' then
         if j < length vs
-        then host_return (s, update_list_at vs j v, RS_normal (vs_to_es ves'))
-        else host_return (s, vs, crash_error)
-      else host_return (s, vs, crash_error)
+        then pure (s, update_list_at vs j v, RS_normal (vs_to_es ves'))
+        else pure (s, vs, crash_error)
+      else pure (s, vs, crash_error)
     | Basic (Tee_local j) =>
       if ves is v :: ves' then
-        host_return (s, vs, RS_normal (vs_to_es (v :: ves) ++ [::Basic (Set_local j)]))
-      else host_return (s, vs, crash_error)
+        pure (s, vs, RS_normal (vs_to_es (v :: ves) ++ [::Basic (Set_local j)]))
+      else pure (s, vs, crash_error)
     | Basic (Get_global j) =>
       if sglob_val s i j is Some xx
-      then host_return (s, vs, RS_normal (vs_to_es (xx :: ves)))
-      else host_return (s, vs, crash_error)
+      then pure (s, vs, RS_normal (vs_to_es (xx :: ves)))
+      else pure (s, vs, crash_error)
     | Basic (Set_global j) =>
       if ves is v :: ves' then
         if supdate_glob s i j v is Some xx
-        then host_return (xx, vs, RS_normal (vs_to_es ves'))
-        else host_return (s, vs, crash_error)
-      else host_return (s, vs, crash_error)
+        then pure (xx, vs, RS_normal (vs_to_es ves'))
+        else pure (s, vs, crash_error)
+      else pure (s, vs, crash_error)
     | Basic (Load t None a off) =>
       if ves is ConstInt32 k :: ves' then
         expect
@@ -381,11 +384,11 @@ with run_one_step (fuel : fuel) (d : depth) (i : instance) (tt : config_one_tupl
                expect
                  (load (mem_s_j) (Wasm_int.nat_of_uint i32m k) off (t_length t))
                  (fun bs =>
-                    host_return (s, vs, RS_normal (vs_to_es (wasm_deserialise bs t :: ves'))))
-                 (host_return (s, vs, RS_normal (vs_to_es ves' ++ [::Trap])))
-             else host_return (s, vs, crash_error))
-          (host_return (s, vs, crash_error))
-      else host_return (s, vs, crash_error)
+                    pure (s, vs, RS_normal (vs_to_es (wasm_deserialise bs t :: ves'))))
+                 (pure (s, vs, RS_normal (vs_to_es ves' ++ [::Trap])))
+             else pure (s, vs, crash_error))
+          (pure (s, vs, crash_error))
+      else pure (s, vs, crash_error)
     | Basic (Load t (Some (tp, sx)) a off) =>
       if ves is ConstInt32 k :: ves' then
         expect
@@ -395,11 +398,11 @@ with run_one_step (fuel : fuel) (d : depth) (i : instance) (tt : config_one_tupl
                expect
                  (load_packed sx (mem_s_j) (Wasm_int.nat_of_uint i32m k) off (tp_length tp) (t_length t))
                  (fun bs =>
-                    host_return (s, vs, RS_normal (vs_to_es (wasm_deserialise bs t :: ves'))))
-                 (host_return (s, vs, RS_normal (vs_to_es ves' ++ [::Trap])))
-             else host_return (s, vs, crash_error))
-          (host_return (s, vs, crash_error))
-      else host_return (s, vs, crash_error)
+                    pure (s, vs, RS_normal (vs_to_es (wasm_deserialise bs t :: ves'))))
+                 (pure (s, vs, RS_normal (vs_to_es ves' ++ [::Trap])))
+             else pure (s, vs, crash_error))
+          (pure (s, vs, crash_error))
+      else pure (s, vs, crash_error)
     | Basic (Store t None a off) =>
       if ves is v :: ConstInt32 k :: ves' then
         if types_agree t v
@@ -411,12 +414,12 @@ with run_one_step (fuel : fuel) (d : depth) (i : instance) (tt : config_one_tupl
                  expect
                    (store mem_s_j (Wasm_int.nat_of_uint i32m k) off (bits v) (t_length t))
                    (fun mem' =>
-                      host_return (upd_s_mem s (update_list_at (s_memory s) j mem'), vs, RS_normal (vs_to_es ves')))
-                   (host_return (s, vs, RS_normal (vs_to_es ves' ++ [::Trap])))
-               else host_return (s, vs, crash_error))
-            (host_return (s, vs, crash_error))
-        else host_return (s, vs, crash_error)
-      else host_return (s, vs, crash_error)
+                      pure (upd_s_mem s (update_list_at (s_memory s) j mem'), vs, RS_normal (vs_to_es ves')))
+                   (pure (s, vs, RS_normal (vs_to_es ves' ++ [::Trap])))
+               else pure (s, vs, crash_error))
+            (pure (s, vs, crash_error))
+        else pure (s, vs, crash_error)
+      else pure (s, vs, crash_error)
     | Basic (Store t (Some tp) a off) =>
       if ves is v :: ConstInt32 k :: ves' then
         if types_agree t v
@@ -428,20 +431,20 @@ with run_one_step (fuel : fuel) (d : depth) (i : instance) (tt : config_one_tupl
                  expect
                    (store_packed mem_s_j (Wasm_int.nat_of_uint i32m k) off (bits v) (tp_length tp))
                    (fun mem' =>
-                      host_return (upd_s_mem s (update_list_at (s_memory s) j mem'), vs, RS_normal (vs_to_es ves')))
-                   (host_return (s, vs, RS_normal (vs_to_es ves' ++ [::Trap])))
-               else host_return (s, vs, crash_error))
-            (host_return (s, vs, crash_error))
-        else host_return (s, vs, crash_error)
-      else host_return (s, vs, crash_error)
+                      pure (upd_s_mem s (update_list_at (s_memory s) j mem'), vs, RS_normal (vs_to_es ves')))
+                   (pure (s, vs, RS_normal (vs_to_es ves' ++ [::Trap])))
+               else pure (s, vs, crash_error))
+            (pure (s, vs, crash_error))
+        else pure (s, vs, crash_error)
+      else pure (s, vs, crash_error)
     | Basic Current_memory =>
       expect
         (smem_ind s i)
         (fun j =>
            if List.nth_error (s_memory s) j is Some s_mem_s_j then
-             host_return (s, vs, RS_normal (vs_to_es (ConstInt32 (Wasm_int.int_of_Z i32m (Z.of_nat (mem_size s_mem_s_j))) :: ves)))
-           else host_return (s, vs, crash_error))
-        (host_return (s, vs, crash_error))
+             pure (s, vs, RS_normal (vs_to_es (ConstInt32 (Wasm_int.int_of_Z i32m (Z.of_nat (mem_size s_mem_s_j))) :: ves)))
+           else pure (s, vs, crash_error))
+        (pure (s, vs, crash_error))
     | Basic Grow_memory =>
       if ves is ConstInt32 c :: ves' then
         expect
@@ -451,11 +454,11 @@ with run_one_step (fuel : fuel) (d : depth) (i : instance) (tt : config_one_tupl
               let: l := mem_size s_mem_s_j in
               let: mem' := mem_grow s_mem_s_j (Wasm_int.nat_of_uint i32m c) in
               let: s' := upd_s_mem s (update_list_at (s_memory s) j mem') in
-              host_return (s', vs, RS_normal (vs_to_es (ConstInt32 (Wasm_int.int_of_Z i32m (Z.of_nat l)) :: ves')))
-            else host_return (s, vs, crash_error))
-          (host_return (s, vs, crash_error))
-      else host_return (s, vs, crash_error)
-    | Basic (EConst _) => host_return (s, vs, crash_error)
+              pure (s', vs, RS_normal (vs_to_es (ConstInt32 (Wasm_int.int_of_Z i32m (Z.of_nat l)) :: ves')))
+            else pure (s, vs, crash_error))
+          (pure (s, vs, crash_error))
+      else pure (s, vs, crash_error)
+    | Basic (EConst _) => pure (s, vs, crash_error)
     | Callcl cl =>
       match cl with
       | Func_native i' (Tf t1s t2s) ts es =>
@@ -465,16 +468,16 @@ with run_one_step (fuel : fuel) (d : depth) (i : instance) (tt : config_one_tupl
         then
           let: (ves', ves'') := split_n ves n in
           let: zs := n_zeros ts in
-          host_return (s, vs, RS_normal (vs_to_es ves''
+          pure (s, vs, RS_normal (vs_to_es ves''
                                 ++ [::Local m i' (rev ves' ++ zs) [::Basic (Block (Tf [::] t2s) es)]]))
-        else host_return (s, vs, crash_error)
+        else pure (s, vs, crash_error)
       | Func_host (Tf t1s t2s) f =>
         let: n := length t1s in
         let: m := length t2s in
         if length ves >= n
         then
-          let: (ves', ves'') := split_n ves n in
-          host_bind (host_apply s f (rev ves')) (fun r =>
+          let (ves', ves'') := split_n ves n in
+          host_apply s f (rev ves') >>= fun r =>
             match r with
             | Some (s', r) =>
               (** We here double-check the types.
@@ -482,55 +485,55 @@ with run_one_step (fuel : fuel) (d : depth) (i : instance) (tt : config_one_tupl
               if result_types_agree t2s r
               then
                 let: rves := result_to_stack r in
-                host_return (s', vs, RS_normal (vs_to_es ves'' ++ rves))
-              else host_return (s, vs, crash_error)
-            | None => host_return (s, vs, crash_error) (* TODO *)
-            end)
-        else host_return (s, vs, crash_error)
+                pure (s', vs, RS_normal (vs_to_es ves'' ++ rves))
+              else pure (s, vs, crash_error)
+            | None => pure (s, vs, crash_error) (* TODO *)
+            end
+        else pure (s, vs, crash_error)
       end
     | Label ln les es =>
       if es_is_trap es
-      then host_return (s, vs, RS_normal (vs_to_es ves ++ [::Trap]))
+      then pure (s, vs, RS_normal (vs_to_es ves ++ [::Trap]))
       else
         if const_list es
-        then host_return (s, vs, RS_normal (vs_to_es ves ++ es))
+        then pure (s, vs, RS_normal (vs_to_es ves ++ es))
         else
-          host_bind (run_step_with_fuel fuel d i (s, vs, es)) (fun rswf =>
+          run_step_with_fuel fuel d i (s, vs, es) >>= fun rswf =>
             let: (s', vs', res) := rswf in
             match res with
             | RS_break 0 bvs =>
               if length bvs >= ln
-              then host_return (s', vs', RS_normal ((vs_to_es ((take ln bvs) ++ ves)) ++ les))
-              else host_return (s', vs', crash_error)
-            | RS_break (n.+1) bvs => host_return (s', vs', RS_break n bvs)
-            | RS_return rvs => host_return (s', vs', RS_return rvs)
+              then pure (s', vs', RS_normal ((vs_to_es ((take ln bvs) ++ ves)) ++ les))
+              else pure (s', vs', crash_error)
+            | RS_break (n.+1) bvs => pure (s', vs', RS_break n bvs)
+            | RS_return rvs => pure (s', vs', RS_return rvs)
             | RS_normal es' =>
-              host_return (s', vs', RS_normal (vs_to_es ves ++ [::Label ln les es']))
-            | RS_crash error => host_return (s', vs', RS_crash error)
-            end)
+              pure (s', vs', RS_normal (vs_to_es ves ++ [::Label ln les es']))
+            | RS_crash error => pure (s', vs', RS_crash error)
+            end
     | Local ln j vls es =>
       if es_is_trap es
-      then host_return (s, vs, RS_normal (vs_to_es ves ++ [::Trap]))
+      then pure (s, vs, RS_normal (vs_to_es ves ++ [::Trap]))
       else
         if const_list es
         then
           if length es == ln
-          then host_return (s, vs, RS_normal (vs_to_es ves ++ es))
-          else host_return (s, vs, crash_error)
+          then pure (s, vs, RS_normal (vs_to_es ves ++ es))
+          else pure (s, vs, crash_error)
         else
-          host_bind (run_step_with_fuel fuel d j (s, vls, es)) (fun rswf =>
+          run_step_with_fuel fuel d j (s, vls, es) >>= fun rswf =>
             let: (s', vls', res) := rswf in
             match res with
             | RS_return rvs =>
               if length rvs >= ln
-              then host_return (s', vs, RS_normal (vs_to_es (take ln rvs ++ ves)))
-              else host_return (s', vs, crash_error)
+              then pure (s', vs, RS_normal (vs_to_es (take ln rvs ++ ves)))
+              else pure (s', vs, crash_error)
             | RS_normal es' =>
-              host_return (s', vs, RS_normal (vs_to_es ves ++ [::Local ln j vls' es']))
-            | RS_crash error => host_return (s', vs, RS_crash error)
-            | RS_break _ _ => host_return (s', vs, crash_error)
-            end)
-    | Trap => host_return (s, vs, crash_error)
+              pure (s', vs, RS_normal (vs_to_es ves ++ [::Local ln j vls' es']))
+            | RS_crash error => pure (s', vs, RS_crash error)
+            | RS_break _ _ => pure (s', vs, crash_error)
+            end
+    | Trap => pure (s, vs, crash_error)
     end
   end.
 
@@ -563,21 +566,21 @@ Fixpoint run_v (fuel : fuel) (d : depth) (i : instance) (tt : config_tuple)
     : host_monad (store_record * res) :=
   let: (s, vs, es) := tt in
   match fuel with
-  | 0 => host_return (s, R_crash C_exhaustion)
+  | 0 => pure (s, R_crash C_exhaustion)
   | fuel.+1 =>
     if es_is_trap es
-    then host_return (s, R_trap)
+    then pure (s, R_trap)
     else
       if const_list es
-      then host_return (s, R_value (fst (split_vals_e es)))
+      then pure (s, R_value (fst (split_vals_e es)))
       else
-        host_bind (run_step d i (s, vs, es)) (fun rs =>
+        run_step d i (s, vs, es) >>= fun rs =>
           let: (s', vs', res) := rs in
           match res with
           | RS_normal es' => run_v fuel d i (s', vs', es')
-          | RS_crash error => host_return (s, R_crash error)
-          | _ => host_return (s, R_crash C_error)
-          end)
+          | RS_crash error => pure (s, R_crash error)
+          | _ => pure (s, R_crash C_error)
+          end
   end.
 
 End Host.
